![[Pasted image 20251029161347.png]]

a, Vorraussetzung
b, Vorraussetzung
c, Behauptung
d, Vorraussetzung
e, Behauptung


![[Pasted image 20251029161719.png]]

Behauptung: $k \mid m \land k \mid n \implies k\mid m+n$
Beweis:
$k \mid m \iff m=k*x_{1},\  x_{i}\in \mathbb{N}$

$k \mid n \iff n=k*x_{2}$
$m+n=k*(x_{1}+x_{2}) \iff m+n \mid k$

![[Pasted image 20251029163642.png]]

a, $\forall x \in \mathbb{P}: x \not \mid 2$, 
Wiederlegung: $2 \in \mathbb{P} \land 2 \mid 2 \implies falsch$ 

b, $k \mid n \land k \mid m \implies k^{2} | n * m$
$\exists n_{0}: n=k*n_{0}$
$\exists m_{0}: m=k*m_{0}$
$k*k \mid k*n_{0}*k*m_{0}$
$1 \mid n_{0}*m_{0}\implies (k \mid n \land k \mid m \implies k^{2} | n * m)$

c, 
$\forall k\forall n\forall m: k \mid m+n \implies k \mid m \lor k \mid n$

Wiederlegung: $k=5, m=3, n=2$ 
$\implies  5\mid 5 w.A.$
$5 \not \mid 3$
$5 \not \mid 2$
=> falsch

