![[Pasted image 20251105161011.png]]


$\left| \frac{x}{y} \right|$

obda.,
$\frac{\left|x \right|}{\left|y \right|}$
$\frac{\left|x \right|}{\left|y \right|}$ x>0 y>0 =$\frac{x}{y}$ 
$\frac{\left|x \right|}{\left|y \right|}$ x<0  y>0= $\frac{-x}{y}<0\implies\frac{\left|-x \right|}{y}>0$
$\frac{\left|x \right|}{\left|y \right|}$ x>0 y<0 => erweitern *-1=> zweiter Fall
$\frac{\left|x \right|}{\left|y \right|}$ x<0 y<0 => erweiter mal -1 => erster Fall

![[Pasted image 20251105162126.png]]

$\forall m,n \in \mathbb{Z}: 2 \not\mid m*n\implies m\not\mid{2} \land n\not\mid{2}$

$\forall m,n \in \mathbb{Z}: m\mid{2} \lor n\mid{2} \implies 2 \mid m*n$
P(m $\lor$ n) = 2*x, x in ZZ
=>m*n=2*x*n

![[Pasted image 20251105162945.png]]
![[Pasted image 20251105163023.png]]
![[Pasted image 20251105163043.png]]

8+3+a=6+2+a=> 11a=8a


